Finish proving [unchanged_payload] in impl

ind/DoublyLinkedList.fst
@@ -1359,7 +1359,7 @@ let _auto_empty_dll (#t:Type) (h0:heap) (d:dll t) :
 
 /// Now for the actual ST operations that will be exposed :)
 
-#set-options "--z3rlimit 500 --max_fuel 2 --max_ifuel 0"
+#set-options "--z3rlimit 500 --max_fuel 2 --max_ifuel 1"
 
 let dll_insert_at_head (#t:Type) (d:dll t) (n:pointer (node t)) :
   StackInline (dll t)
@@ -1372,6 +1372,7 @@ let dll_insert_at_head (#t:Type) (d:dll t) (n:pointer (node t)) :
                          (Mod.loc_buffer n)
                          (Mod.loc_buffer d.lhead)) h0 h1 /\
          dll_valid h1 y /\
+         unchanged_node_vals h0 h1 (reveal y.nodes) /\
          reveal y.nodes == n :: reveal d.nodes)) =
   if is_null d.lhead then (
     singleton_dll n
@@ -1384,6 +1385,10 @@ let dll_insert_at_head (#t:Type) (d:dll t) (n:pointer (node t)) :
     let h0' = ST.get () in
     n <|= h;
     let h1 = ST.get () in
+    //
+    let rec unchanged_payload nl : Lemma (unchanged_node_vals h0 h1 nl) =
+      if (length nl = 0) then () else unchanged_payload (tl nl) in
+    unchanged_payload (reveal d.nodes);
     //
     let Frag1 p1 = tot_dll_to_fragment h0 d in
     let p = tot_node_to_piece h0 n in
